proof/proof/alicebob.v
@@ -1,6 +1,47 @@
 From New.generatedproof.github_com.sanjit_bhat.pav Require Import alicebob.
 From New.proof.github_com.sanjit_bhat.pav Require Import prelude.
 
+From New.proof Require Import bytes time.
+From New.proof.github_com.goose_lang Require Import primitive std.
 From New.proof.github_com.sanjit_bhat.pav Require Import
-  advrpc auditor client cryptoffi cryptoutil hashchain ktcore
-  merkle netffi safemarshal server.
+  auditor client cryptoffi ktcore server.
+
+Module alicebob.
+
+Module Trust.
+Inductive t :=
+  | No
+  | SigPred
+  | Full.
+
+Definition rank t : nat :=
+  match t with No => 0 | SigPred => 1 | Full => 2 end.
+End Trust.
+
+Section proof.
+Context `{!heapGS Σ}.
+Context {sem : go.Semantics} {package_sem : alicebob.Assumptions}.
+Collection W := sem + package_sem.
+#[local] Set Default Proof Using "W".
+
+#[global] Instance : IsPkgInit (iProp Σ) alicebob := define_is_pkg_init True%I.
+#[global] Instance : GetIsPkgInitWf (iProp Σ) alicebob := build_get_is_pkg_init_wf.
+
+(* [alice_okay] is whether alice's uid is adversarially controlled. *)
+Lemma wp_testAliceBob (serv_trust adtr_trust : Trust.t)
+    (alice_okay bob_okay : bool)
+    (servAddr : w64) (servGood : bool) sl_adtrAddrs (adtrAddrs : list w64) :
+  {{{
+    is_pkg_init alicebob ∗
+    "#Hsl_adtrAddrs" ∷ sl_adtrAddrs ↦*□ adtrAddrs ∗
+    "%Heq_servGood" ∷ ⌜servGood =
+      bool_decide (Trust.rank Trust.No < Trust.rank serv_trust)⌝ ∗
+    "%Hmin_trust" ∷ ⌜Trust.rank Trust.No < Trust.rank serv_trust ∨
+      Trust.rank Trust.No < Trust.rank adtr_trust⌝
+  }}}
+  @! alicebob.testAliceBob #servAddr #servGood #sl_adtrAddrs
+  {{{ RET #(); True }}}.
+Proof. Admitted.
+
+End proof.
+End alicebob.
